Coroutine.v
@@ -1,0 +1,239 @@
+Require Import List.
+Import ListNotations.
+Require Import Bool.
+Require Import Coq.Logic.FunctionalExtensionality.
+Require Import Omega.
+Require Import Trace.
+Require Import Machine.
+Require Import ObsTrace.
+
+(* A Domain is an annotation on a component or set of components reflecting its
+   relationship to the program state. Domains are nested, so a domain can be subsumed by
+   a higher domain, and all of its components with it. For instance, a stack in a coroutine
+   system has a domain containing all of the addresses in the stack's range, and the frames
+   pushed on the stack each have their own, as described below. *)
+Section DOMAIN_MODEL.
+
+  Inductive ShareStatus :=
+  | Local
+  | Shared
+  | Passed
+  .
+  
+  Inductive StackDomain :=
+  | Inactive (sd:StackDomain) (ss:ShareStatus)
+  | Active (ss:ShareStatus)
+  .
+
+  Definition statusOf sd :=
+    match sd with
+    | Inactive _ ss => ss
+    | Active ss => ss
+    end.
+
+  Inductive TopDomain :=
+  | Instack (sid:StackID) (sd:StackDomain)
+  | Other
+  .
+
+  (* Finally we need a way to map components to the domain they belong to. *)
+  Definition DomainMap := Component -> TopDomain.
+  Definition DepthMap := StackID -> nat.
+  Definition initDepM : DepthMap := fun sid => O.
+  Definition push (depm: DepthMap) (sid: StackID) :=
+    fun sid' => if stack_eqb sid sid'
+                then (depm sid)+1
+                else depm sid.
+  Definition pop (depm: DepthMap) (sid: StackID) :=
+    fun sid' => if stack_eqb sid sid'
+                then (depm sid)-1
+                else depm sid.
+  
+End DOMAIN_MODEL.
+
+Section WITH_MAPS.
+
+  Variable cdm : CodeMap'.
+  Variable sm : StackMap.
+  Variable pOf : MachineState -> PolicyState.
+  
+  Definition initD : DomainMap * DepthMap :=
+    let dm := fun k =>
+                match k with
+                | Mem a =>
+                  match findStack sm a with
+                  | Some sid => Instack sid (Active Local)
+                  | None => Other
+                  end
+                | Reg r => Other
+                end in
+    (dm,initDepM).
+  
+  (* Our update function checks an "annotation" on the code being executed.
+     Annotations are defined in Machine.v as an alternative to a million different
+     maps, and the ones that matter are call, return, yield, and share.
+
+     Annotations are given by the compiler. We assume that the compiler can tell us
+     which instructions represent calls, returns, and yields. Shares are more complicated;
+     the compiler cannot directly tell us which component(s) are being shared, because sharing
+     is often dynamic. What it can do is identify a relation between the machine state
+     and the component(s) being shared.
+     
+     For an example, suppose that a caller is sharing an address as an argument to its callee.
+     It executes a store instruction that the compiler identifies as a share; the target of
+     the share is the address to which the argument is being stored, held within the appropriate
+     register. So, we would relate a given machine state to the contents of the register in that
+     state.
+     
+     This is a much stronger assumption of information from the compiler than we had before!
+     We now fully rely on the compiler to recognize returns, for instance. Relating returns
+     to the actual program state is the job of control flow property, WBCF.
+
+     Note that yields don't actually change the domain map, as they don't change which
+     addresses belong to which stacks. *)
+  
+  Definition updateD (m:MachineState) (prev:DomainMap*DepthMap) : DomainMap * DepthMap :=
+    let '(dm, depm) := prev in
+    match AnnotationOf cdm (m (Reg PC)), findStack sm (m (Reg SP)) with
+    | Some call, Some sid => (* A call adjusts the domain map by marking the caller's frame "inactive" *)
+                   (* and wrapping the remaining stack in a new instance of "active" *)
+      let dm' := fun k =>
+                   match k, dm k with
+                   | _, Other => Other
+                   | Mem a, Instack sid (Active ss) =>
+                     if wlt a (m (Reg SP))
+                     then Instack sid (Inactive (Active ss) ss)
+                     else Instack sid (Active ss)
+                   | Mem a, Instack sid (Inactive sd Passed) =>
+                     Instack sid (Inactive (Inactive sd Passed) Local)
+                   | Mem a, Instack sid (Inactive sd ss) =>
+                     Instack sid (Inactive (Inactive sd ss) ss)
+                   | _, _ => dm k
+                   end in
+      (dm', push depm sid)
+    | Some ret, Some sid => (* A return unwraps the outermost domain of all components in the initial stack *)
+      let dm' := fun k =>
+                   match dm k with
+                   | Instack sid (Inactive sd Passed) => Instack sid (Active Local)
+                   | Instack sid (Inactive sd ss) => Instack sid sd
+                   | _ => dm k
+                   end in
+      (dm', pop depm sid)
+    | _,_ => (dm,depm)
+    end.
+
+  Definition StackIntegrityUE : Prop :=
+    forall minit MCP k sid sd mcp mcp',
+      WithContextMP updateD initD (MPTraceOf (minit, pOf minit)) MCP ->
+      ContextSegment (fun _ _ => False) MCP (notfinished mcp (finished mcp')) ->
+      fst (cstate mcp) k = Instack sid (Inactive sd Local) ->
+      mstate mcp k = mstate mcp' k.
+
+    (* We can do a similar Ultra Eager style property with confidentiality, and since we're
+       not allowing sharing it is straightforward. But some preliminaries on confidentiality.
+       Firstly: confidentiality is expressed in terms of "variant" states. A K-variant
+       state of m is a state that agrees with m at every component not in the set K. It may also
+       agree at some components in K. The intuition is that if the step from a state changes the
+       state in the same way as the step from its K-variant, we can't tell from that step what
+       value a component in K was, so K is secret. *)
+  Definition variantOf (K : Component -> Prop) (m n : MachineState) :=
+    forall k, ~ K k -> m k = n k.
+  
+  (* "Changing the state in the same way" means that any component that changed is
+     one trace ends with the same value in the other. *)
+  Definition sameDifference (m m' n n' : MachineState) :=
+    forall k,
+      (m k <> m' k \/ n k <> n' k) ->
+      m' k = n' k.
+  
+  Definition StackConfidentialityUE : Prop :=
+    forall minit MCP sid sd mcp mcp' n n' o,
+      WithContextMP updateD initD (MPTraceOf (minit, pOf minit)) MCP ->
+      ContextSegment (fun _ _ => False) MCP (notfinished mcp (finished mcp')) ->
+      variantOf (fun k => fst (cstate mcp) k = Instack sid (Inactive sd Local)) (mstate mcp) n ->
+      step (mstate mcp) = (mstate mcp', o) ->
+      step n = (n',o) /\ sameDifference (mstate mcp) (mstate mcp') n n'.
+
+  Definition FindSegmentMP P mp dm MCP :=
+    exists MCP',
+      WithContextMP updateD dm (MPTraceOf mp) MCP' /\
+      ContextSegment P MCP' MCP.
+
+  Definition FindSegmentM P m dm MC :=
+    exists MC',
+      WithContextM updateD dm (MTraceOf m) MC' /\
+      ContextSegmentM P MC' MC.
+  
+  Definition StackIntegrityEager : Prop :=
+    forall minit MCP d k sid sd mcp mcp',
+      FindSegmentMP  (fun m c => snd c = d) (minit, pOf minit) initD MCP ->
+      mcp = head MCP ->
+      fst (cstate mcp) k = Instack sid (Inactive sd Local) ->
+      Last MCP mcp' ->
+      mstate mcp k = mstate mcp' k.
+  
+  Definition Stuck (MCP : @MCPTrace (DomainMap * DepthMap)) : Prop :=
+    exists m c p,
+      Last MCP (m,c,p) ->
+      mpstep (m,p) = None.
+
+  Definition StackConfidentialityEager : Prop :=
+    forall minit M MO d sid sd m dm depm p n N NO,
+      let P := (fun m c => snd c sid = d) in
+      FindSegmentMP P (minit, pOf minit) initD M ->
+      head M = (m,(dm,depm),p) ->
+      variantOf (fun k => dm k = Instack sid (Inactive sd Local)) m n ->
+      FindSegmentM P n (dm,depm) N ->
+      ObsOfMCP M MO ->
+      ObsOfMC N NO ->
+         (* Case 1 *)
+      (forall mend dmend depmend pend,
+          Last M (mend,(dmend,depmend),pend) ->
+          ~ P mend (dm,depm) ->
+          exists nend dnend,
+            Last N (nend,dnend) /\
+            ObsOfMP MO ~=_O ObsOfM NO /\
+            sameDifference m mend n nend)
+      /\ (* Case 2 *)
+      (Infinite M ->
+       ObsOfMP MO ~=_O ObsOfM NO)
+      /\ (* Case 3 *)
+      (Stuck M ->
+       ObsOfMP MO <=_O ObsOfM NO).
+
+  Inductive StepsTo : MachineState -> MachineState -> Prop :=
+  | isNow : forall m, StepsTo m m
+  | stepsTo : forall m1 m2 m' o,
+      step m1 = (m',o) ->
+      StepsTo m' m2 ->
+      StepsTo m1 m2.
+
+  Definition CallRule : Prop :=
+    forall minit MCP mcall dmcall depmcall pcall sid,
+      WithContextMP updateD initD (MPTraceOf (minit, pOf minit)) MCP ->
+      InTrace (mcall,(dmcall,depmcall),pcall) MCP ->
+      AnnotationOf cdm (mcall (Reg PC)) = Some call ->
+      findStack sm (mcall (Reg SP)) = Some sid ->
+         (* Case 1: Divergence (including due to failstop) *)
+      (forall MCP' m' dm d p',
+          WithContextMP updateD (dmcall,depmcall) (MPTraceOf (mcall,pcall)) MCP' ->
+          InTrace (m',dm,p') MCP' ->
+          d > depmcall sid)
+      \/ (* Case 2: Return *)
+      (exists m',
+          StepsTo mcall m' /\
+          (forall k sid sd,
+            dmcall k = Instack sid (Inactive sd Local) ->
+            mcall k = m' k) /\
+          (forall n k,
+              variantOf (fun k' => exists sid sd, dmcall k = Instack sid (Inactive sd Local)) mcall n ->
+              StepsTo n m')).
+
+  Theorem EagerSufficient :
+    StackIntegrityEager ->
+    StackConfidentialityEager ->
+    CallRule.
+  Proof.
+  Admitted.
+
+End WITH_MAPS.
