Makefile
@@ -15,4 +15,4 @@ coq:
 	coqc -R . "" formal.v
 
 clean:
-	rm -f *.aux
+	rm -f *.aux *.vio *.vo* *.glob
